FGL: improve proof scheme for meta rules

books/centaur/fgl/primitives-stub.lisp
@@ -309,26 +309,64 @@
 
 (set-state-ok t)
 
+(define implies* (x y)
+  :no-function t
+  (implies x y)
+  ///
+  (defthm implies*-of-nil
+    (implies* nil x))
+
+  (defthm implies*-of-t
+    (iff (implies* t x) x))
+
+  (defthm implies*-x-nil
+    (iff (implies* x nil)
+         (not x)))
+
+  (defthm implies*-x-t
+    (implies* x t))
+
+  (defcong iff equal (implies* x y) 1)
+  (defcong iff equal (implies* x y) 2))
+
+(define not* (x)
+  :no-function t
+  (not x)
+  ///
+  (defcong iff equal (not* x) 1))
+
+(local (in-theory (enable implies* not*)))
+
+(defmacro <=* (x y) `(not* (< ,y ,x)))
+(defmacro >=* (x y) `(not* (< ,x ,y)))
+
 (make-event
  (let ((body `(b* (((mv successp ans new-interp-st new-state) result))
-                (and ,@(strip-cars (strip-cdrs (strip-cdrs *fgl-primitive-rule-thms*)))
-                     (implies (and successp
-                                   (equal contexts (interp-st->equiv-contexts interp-st))
-                                   (fgl-ev-meta-extract-global-facts :state st)
-                                   formula-check
-                                   (equal (w st) (w state))
-                                   (interp-st-bfrs-ok interp-st)
-                                   (interp-st-bfr-listp (fgl-objectlist-bfrlist args))
-                                   (logicman-pathcond-eval (fgl-env->bfr-vals env)
-                                                           (interp-st->constraint interp-st)
-                                                           (interp-st->logicman interp-st))
-                                   (logicman-pathcond-eval (fgl-env->bfr-vals env)
-                                                           (interp-st->pathcond interp-st)
-                                                           (interp-st->logicman interp-st)))
-                              (equal (fgl-ev-context-fix contexts
-                                                         (fgl-object-eval ans env (interp-st->logicman new-interp-st)))
-                                     (fgl-ev-context-fix contexts
-                                                         (fgl-object-eval (g-apply origfn args) env (interp-st->logicman interp-st)))))))))
+                (and* ,@(sublis '((implies . implies*)
+                                  (and . and*)
+                                  (not . not*)
+                                  (iff . iff*)
+                                  (or . or*)
+                                  (<= . <=*)
+                                  (>= . >=*))
+                                (strip-cars (strip-cdrs (strip-cdrs *fgl-primitive-rule-thms*))))
+                      (implies* (and* successp
+                                     (equal contexts (interp-st->equiv-contexts interp-st))
+                                     (fgl-ev-meta-extract-global-facts :state st)
+                                     formula-check
+                                     (equal (w st) (w state))
+                                     (interp-st-bfrs-ok interp-st)
+                                     (interp-st-bfr-listp (fgl-objectlist-bfrlist args))
+                                     (logicman-pathcond-eval (fgl-env->bfr-vals env)
+                                                             (interp-st->constraint interp-st)
+                                                             (interp-st->logicman interp-st))
+                                     (logicman-pathcond-eval (fgl-env->bfr-vals env)
+                                                             (interp-st->pathcond interp-st)
+                                                             (interp-st->logicman interp-st)))
+                                (equal (fgl-ev-context-fix contexts
+                                                           (fgl-object-eval ans env (interp-st->logicman new-interp-st)))
+                                       (fgl-ev-context-fix contexts
+                                                           (fgl-object-eval (g-apply origfn args) env (interp-st->logicman interp-st)))))))))
    `(progn (defconst *fgl-primitive-constraint-base-body* ',body)
            (defun-nx fgl-primitive-constraint-base (result
                                                     origfn args interp-st state
@@ -374,30 +412,37 @@
 
 (make-event
  (let ((body `(b* (((mv successp rhs bindings new-interp-st new-state) result))
-                (and ,@(strip-cars (strip-cdrs (strip-cdrs *fgl-meta-rule-thms*)))
-                     (implies (and successp
-                                   (equal contexts (interp-st->equiv-contexts interp-st))
-                                   (fgl-ev-meta-extract-global-facts :state st)
-                                   formula-check
-                                   (equal (w st) (w state))
-                                   (interp-st-bfrs-ok interp-st)
-                                   (interp-st-bfr-listp (fgl-objectlist-bfrlist args))
-                                   (logicman-pathcond-eval (fgl-env->bfr-vals env)
-                                                           (interp-st->constraint interp-st)
-                                                           (interp-st->logicman interp-st))
-                                   (logicman-pathcond-eval (fgl-env->bfr-vals env)
-                                                           (interp-st->pathcond interp-st)
-                                                           (interp-st->logicman interp-st))
-                                   (pseudo-fnsym-p origfn))
-                              (fgl-ev-context-equiv-forall-extensions
-                               contexts
-                               (fgl-ev (cons origfn (kwote-lst
-                                                     (fgl-objectlist-eval
-                                                      args env
-                                                      (interp-st->logicman interp-st))))
-                                       nil)
-                               rhs
-                               (fgl-object-bindings-eval bindings env (interp-st->logicman new-interp-st))))))))
+                (and* ,@(sublis '((implies . implies*)
+                                  (and . and*)
+                                  (not . not*)
+                                  (iff . iff*)
+                                  (or . or*)
+                                  (<= . <=*)
+                                  (>= . >=*))
+                                (strip-cars (strip-cdrs (strip-cdrs *fgl-meta-rule-thms*))))
+                      (implies* (and* successp
+                                     (equal contexts (interp-st->equiv-contexts interp-st))
+                                     (fgl-ev-meta-extract-global-facts :state st)
+                                     formula-check
+                                     (equal (w st) (w state))
+                                     (interp-st-bfrs-ok interp-st)
+                                     (interp-st-bfr-listp (fgl-objectlist-bfrlist args))
+                                     (logicman-pathcond-eval (fgl-env->bfr-vals env)
+                                                             (interp-st->constraint interp-st)
+                                                             (interp-st->logicman interp-st))
+                                     (logicman-pathcond-eval (fgl-env->bfr-vals env)
+                                                             (interp-st->pathcond interp-st)
+                                                             (interp-st->logicman interp-st))
+                                     (pseudo-fnsym-p origfn))
+                                (fgl-ev-context-equiv-forall-extensions
+                                 contexts
+                                 (fgl-ev (cons origfn (kwote-lst
+                                                       (fgl-objectlist-eval
+                                                        args env
+                                                        (interp-st->logicman interp-st))))
+                                         nil)
+                                 rhs
+                                 (fgl-object-bindings-eval bindings env (interp-st->logicman new-interp-st))))))))
    `(progn
       (defconst *fgl-meta-constraint-base-body* ',body)
       (defun-nx fgl-meta-constraint-base (result
@@ -449,8 +494,15 @@
 
 (make-event
  (let ((body `(b* (((mv successp rhs bindings rhs-contexts new-interp-st new-state) result))
-                (and ,@(strip-cars (strip-cdrs (strip-cdrs *fgl-binder-rule-thms*)))
-                     (implies (and successp
+                (and* ,@(sublis '((implies . implies*)
+                                  (and . and*)
+                                  (not . not*)
+                                  (iff . iff*)
+                                  (or . or*)
+                                  (<= . <=*)
+                                  (>= . >=*))
+                                (strip-cars (strip-cdrs (strip-cdrs *fgl-binder-rule-thms*))))
+                     (implies* (and* successp
                                    (equal contexts (interp-st->equiv-contexts interp-st))
                                    (fgl-ev-meta-extract-global-facts :state st)
                                    formula-check
@@ -720,12 +772,165 @@
                        (equal (w st) (w state)))
                   (fgl-formula-checks-stub state))))
 
+(defsection and*-split-clause-proc
+  (defevaluator and*-ev and*-ev-list ((acl2::binary-and* x y) (if a b c) (not x) (equal x y) (implies x y)) :namedp t)
+  (local (acl2::def-join-thms and*-ev))
+
+  (local (acl2::def-ev-pseudo-term-fty-support and*-ev and*-ev-list))
+
+  (define lambda-calls-from-bodies ((formals symbol-listp)
+                                   (bodies pseudo-term-listp)
+                                   (args pseudo-term-listp))
+    :guard (eql (len formals) (len args))
+    :hooks nil
+    :returns (lambdas pseudo-term-listp)
+    (if (atom bodies)
+        nil
+      (cons (pseudo-term-lambda formals (car bodies) args)
+            (lambda-calls-from-bodies formals (cdr bodies) args)))
+    ///
+    (defret and*-ev-of-conjoin-<fn>
+      (iff (and*-ev (conjoin lambdas) env)
+           (and*-ev (conjoin bodies) (pairlis$ formals (and*-ev-list args env))))))
+
+  (define split-and* ((x pseudo-termp))
+    :returns (conj pseudo-term-listp)
+    :measure (pseudo-term-count x)
+    :verify-guards nil
+    (pseudo-term-case x
+      :fncall (cond ((eq x.fn 'acl2::binary-and*)
+                     (append (split-and* (first x.args))
+                             (split-and* (second x.args))))
+                    ((and (eq x.fn 'acl2::if)
+                          (equal (third x.args) ''nil))
+                     (append (split-and* (first x.args))
+                             (split-and* (second x.args))))
+                    (t (list (pseudo-term-fix x))))
+      :lambda (lambda-calls-from-bodies x.formals (split-and* x.body) x.args)
+      :otherwise (list (pseudo-term-fix x)))
+    ///
+    (verify-guards split-and*)
+    
+    (local (defun-sk and*-ev-of-split-and-cond (x)
+             (forall env
+                     (iff (and*-ev (conjoin (split-and* x)) env)
+                          (and*-ev x env)))
+             :rewrite :direct))
+    (local (in-theory (disable and*-ev-of-split-and-cond)))
+    (local (defthm and*-ev-of-split-and-lemma
+             (and*-ev-of-split-and-cond x)
+             :hints (("goal" :induct (split-and* x))
+                     (and stable-under-simplificationp
+                          `(:expand (,(car (last clause))))))))
+    (defthm and*-ev-of-split-and
+      (iff (and*-ev (conjoin (split-and* x)) env)
+           (and*-ev x env))))
+
+  (local (defthm and*-ev-disjoin-pseudo-term-list-fix
+           (iff (and*-ev (disjoin (pseudo-term-list-fix x)) a)
+                (and*-ev (disjoin x) a))
+           :hints(("Goal" :in-theory (enable pseudo-term-list-fix)
+                   :induct (len x)))))
+
+  (define add-last-clauses ((prev pseudo-term-listp) (lasts pseudo-term-listp))
+    :returns (clauses pseudo-term-list-listp)
+    (if (atom lasts)
+        nil
+      (cons (append (pseudo-term-list-fix prev)
+                    (list (pseudo-term-fix (car lasts))))
+            (add-last-clauses prev (cdr lasts))))
+    ///
+    (defthm conjoin-clauses-of-add-last-clauses
+      (iff (and*-ev (conjoin-clauses (add-last-clauses prev lasts)) env)
+           (or (and*-ev (disjoin prev) env)
+               (and*-ev (conjoin lasts) env)))))
+  
+  (local (defthm and*-ev-of-disjoin-take
+           (implies (not (and*-ev (disjoin x) a))
+                    (not (and*-ev (disjoin (take n x)) a)))))
+
+  (local (defthm and*-ev-of-car-last
+           (implies (not (and*-ev (disjoin x) a))
+                    (not (and*-ev (car (last x)) a)))))
+
+  (define and*-split-clause-proc ((clause pseudo-term-listp))
+    :hooks nil
+    (b* ((last (car (last clause)))
+         (prev (butlast clause 1)))
+      (add-last-clauses prev (split-and* last)))
+    ///
+    (defthm and*-split-clause-proc-correct
+      (implies (and (pseudo-term-listp clause)
+                    (alistp a)
+                    (and*-ev (conjoin-clauses (and*-split-clause-proc clause)) a))
+               (and*-ev (disjoin clause) a))
+      :rule-classes :clause-processor))
+
+  (local (defthm and*ev-dumb-negate-lit-correct
+           (implies (pseudo-termp x)
+                    (iff (and*-ev (acl2::dumb-negate-lit x) a)
+                         (not (and*-ev x a))))
+           :hints(("Goal" :in-theory (enable acl2::dumb-negate-lit)))))
+
+
+  (verify-termination acl2::dumb-negate-lit-lst)
+
+
+  (local (defthm and*-ev-disjoin-dumb-negate-lit-list
+           (implies (pseudo-term-listp x)
+                    (iff (and*-ev (disjoin (acl2::dumb-negate-lit-lst x)) a)
+                         (not (and*-ev (conjoin x) a))))
+           :hints(("Goal" :in-theory (enable acl2::dumb-negate-lit-lst)))))
+
+  (local (defthm pseudo-term-listp-of-dumb-negate-lit-lst
+           (implies (pseudo-term-listp x)
+                    (pseudo-term-listp (acl2::dumb-negate-lit-lst x)))
+           :hints(("Goal" :in-theory (enable acl2::dumb-negate-lit-lst)))))
+
+  (define flatten-and*-hyps ((clause pseudo-term-listp))
+    :returns (new-clause pseudo-term-listp)
+    (b* (((when (atom clause)) nil)
+         (lit (car clause)))
+      (pseudo-term-case lit
+        :fncall (cond ((eq lit.fn 'not)
+                       (append (ec-call (acl2::dumb-negate-lit-lst (split-and* (first lit.args))))
+                               (flatten-and*-hyps (cdr clause))))
+                      ((eq lit.fn 'implies)
+                       (append (ec-call (acl2::dumb-negate-lit-lst (split-and* (first lit.args))))
+                               (cons (second lit.args)
+                                     (flatten-and*-hyps (cdr clause)))))
+                      (t (cons (pseudo-term-fix lit) (flatten-and*-hyps (cdr clause)))))
+        :otherwise
+        (cons (pseudo-term-fix lit) (flatten-and*-hyps (cdr clause)))))
+    ///
+    (defthm and*-ev-of-flatten-and*-hyps
+      (iff (and*-ev (disjoin (flatten-and*-hyps clause)) a)
+           (and*-ev (disjoin clause) a))))
+
+  (define flatten-and*-clause-proc ((clause pseudo-term-listp))
+    (list (flatten-and*-hyps clause))
+    ///
+    (defthm flatten-and*-clause-proc-correct
+      (implies (and (pseudo-term-listp clause)
+                    (alistp a)
+                    (and*-ev (conjoin-clauses (flatten-and*-clause-proc clause)) a))
+               (and*-ev (disjoin clause) a))
+      :rule-classes :clause-processor)))
+
 
 
 (defsection fgl-primitive-fncall-stub
   (local (std::set-define-current-function fgl-primitive-fncall-stub))
   ;; (local (defthm iff-is-iff*
   ;;          (equal (iff x y) (iff* x y))))
+  ;; (local
+  ;;  #!acl2
+  ;;  (progn (defun quick-and-dirty-srs-off (cl1 ac)
+  ;;           (declare (ignore cl1 ac)
+  ;;                    (xargs :mode :logic :guard t))
+  ;;           nil)
+
+  ;;         (defattach-system quick-and-dirty-srs quick-and-dirty-srs-off)))
   (local
    (make-event
     `(progn
@@ -749,10 +954,33 @@
                    mode env n contexts st)
                   ,(sublis '((result . (fgl-primitive-fncall-stub
                                         primfn origfn args interp-st state))
-                             (formula-check . (fgl-formula-checks-stub state)))
+                             (formula-check . (fgl-formula-checks-stub state))
+                             (and* . and)
+                             (implies* . implies)
+                             (not* . not)
+                             (or* . or)
+                             (<=* . <=)
+                             (>=* . >=))
                           (remove-bind-free *fgl-primitive-constraint-base-body*)))
-         :hints (("goal" :in-theory '(fgl-primitive-constraint-base)
-                  :do-not '(preprocess)))))))
+         :hints (("goal" :clause-processor (flatten-and*-clause-proc clause)
+                  :in-theory '(fgl-primitive-constraint-base))
+                 '(:clause-processor (and*-split-clause-proc clause))
+                 '(:in-theory '(fgl-primitive-constraint-base
+                                implies*-of-nil implies*-of-t implies*-x-nil implies*-x-t
+                                acl2::and*-rem-first acl2::and*-rem-second
+                                acl2::and*-nil-first acl2::and*-nil-second
+                                iff-implies-equal-implies*-1
+                                iff-implies-equal-implies*-2
+                                iff-implies-equal-not*-1
+                                acl2::iff-implies-equal-and*-1
+                                acl2::iff-implies-iff-and*-2
+                                (not*))
+                   :do-not '(preprocess)
+                   ;; :case-split-limitations (10 10)
+                   )
+                 (and stable-under-simplificationp
+                      '(:clause-processor (flatten-and*-clause-proc clause)))
+                 )))))
   
   (set-default-hints
    '('(:use ((:instance fgl-primitive-constraint-necc
@@ -829,10 +1057,33 @@
                    mode env n contexts st)
                   ,(sublis '((result . (fgl-meta-fncall-stub
                                         primfn origfn args interp-st state))
-                             (formula-check . (fgl-formula-checks-stub state)))
+                             (formula-check . (fgl-formula-checks-stub state))
+                             (and* . and)
+                             (implies* . implies)
+                             (not* . not)
+                             (or* . or)
+                             (<=* . <=)
+                             (>=* . >=))
                            (remove-bind-free *fgl-meta-constraint-base-body*)))
-         :hints (("goal" :in-theory '(fgl-meta-constraint-base)
-                  :do-not '(preprocess)))))))
+         :hints (("goal" :clause-processor (flatten-and*-clause-proc clause)
+                  :in-theory '(fgl-meta-constraint-base))
+                 '(:clause-processor (and*-split-clause-proc clause))
+                 '(:in-theory '(fgl-meta-constraint-base
+                                implies*-of-nil implies*-of-t implies*-x-nil implies*-x-t
+                                acl2::and*-rem-first acl2::and*-rem-second
+                                acl2::and*-nil-first acl2::and*-nil-second
+                                iff-implies-equal-implies*-1
+                                iff-implies-equal-implies*-2
+                                iff-implies-equal-not*-1
+                                acl2::iff-implies-equal-and*-1
+                                acl2::iff-implies-iff-and*-2
+                                (not*))
+                   :do-not '(preprocess)
+                   ;; :case-split-limitations (10 10)
+                   )
+                 (and stable-under-simplificationp
+                      '(:clause-processor (flatten-and*-clause-proc clause)))
+                 )))))
   
   (set-default-hints
    '('(:use ((:instance fgl-meta-constraint-necc
@@ -912,10 +1163,33 @@
                    mode env n contexts st rhs-val eval-alist)
                   ,(sublis '((result . (fgl-binder-fncall-stub
                                         primfn origfn args interp-st state))
-                             (formula-check . (fgl-formula-checks-stub state)))
+                             (formula-check . (fgl-formula-checks-stub state))
+                             (and* . and)
+                             (implies* . implies)
+                             (not* . not)
+                             (or* . or)
+                             (<=* . <=)
+                             (>=* . >=))
                            (remove-bind-free *fgl-binder-constraint-base-body*)))
-         :hints (("goal" :in-theory '(fgl-binder-constraint-base)
-                  :do-not '(preprocess)))))))
+         :hints (("goal" :clause-processor (flatten-and*-clause-proc clause)
+                  :in-theory '(fgl-binder-constraint-base))
+                 '(:clause-processor (and*-split-clause-proc clause))
+                 '(:in-theory '(fgl-binder-constraint-base
+                                implies*-of-nil implies*-of-t implies*-x-nil implies*-x-t
+                                acl2::and*-rem-first acl2::and*-rem-second
+                                acl2::and*-nil-first acl2::and*-nil-second
+                                iff-implies-equal-implies*-1
+                                iff-implies-equal-implies*-2
+                                iff-implies-equal-not*-1
+                                acl2::iff-implies-equal-and*-1
+                                acl2::iff-implies-iff-and*-2
+                                (not*))
+                   :do-not '(preprocess)
+                   ;; :case-split-limitations (10 10)
+                   )
+                 (and stable-under-simplificationp
+                      '(:clause-processor (flatten-and*-clause-proc clause)))
+                 )))))
   
   (set-default-hints
    '('(:use ((:instance fgl-binder-constraint-necc
